Fix deleted id sets (#20)
* fixing

* introduce deletedIdSets

* fix commutativity

* wip

* insert/delete

* remove comment

* fix sorries

* fix

* done

LeanYjs/Algorithm/Delete/Basic.lean
@@ -1,29 +1,7 @@
 import LeanYjs.Item
-import LeanYjs.Algorithm.Invariant.Basic
-import LeanYjs.Algorithm.Invariant.YjsArray
+import LeanYjs.Algorithm.Basic
 
-mutual
-def deleteItemById (item : YjsItem A) (id : YjsId) : YjsItem A :=
-  match item with
-  | YjsItem.mk o r iid c d =>
-    if iid = id then
-      YjsItem.mk (deletePtrById o id) (deletePtrById r id) iid c true
-    else
-      YjsItem.mk (deletePtrById o id) (deletePtrById r id) iid c d
-
-def deletePtrById (ptr : YjsPtr A) (id : YjsId) : YjsPtr A :=
-  match ptr with
-  | YjsPtr.itemPtr item => YjsPtr.itemPtr (deleteItemById item id)
-  | YjsPtr.first => YjsPtr.first
-  | YjsPtr.last => YjsPtr.last
-end
-
-/--
-  Delete the item with the given id from the array by marking it as deleted.
-  Not only the item itself but also all its origins and right origins are marked as deleted.
-  This is done to maintain the invariants of the Yjs array.
-  In real Yjs implementation, it just change the field and does not traverse the origins because the origin/rightOrigins are references to other items.
--/
-def deleteById (arr : Array (YjsItem A)) (id : YjsId) : Array (YjsItem A) :=
-  -- Mark the item with the given id as deleted
-  arr.map fun item => deleteItemById item id
+def deleteById (state : YjsState A) (id : YjsId) : YjsState A :=
+  { state with
+      deletedIds := state.deletedIds.insert id
+  }
