LeanYjs/Algorithm/Insert/Spec.lean
@@ -131,7 +131,7 @@ omit [DecidableEq A] in theorem not_rightOrigin_first (P : YjsPtr A -> Prop) (it
   intros hclosed hinv hin heq
   have hlt : YjsLt' (A := A) item item.rightOrigin := by
     exists 1
-    obtain ⟨ o, r, id, c, d ⟩ := item
+    obtain ⟨ o, r, id, c ⟩ := item
     apply YjsLt.ltRightOrigin
     left
   obtain ⟨ _, hlt ⟩ := hlt
@@ -215,7 +215,7 @@ theorem loopInv_YjsLt' {current} offset (arr : Array (YjsItem A)) (newItem : Yjs
 
         have hsize : ro.size < arr[j].size := by
           revert h_ro_eq
-          obtain ⟨ o, r, id, c, d ⟩ := arr[j]
+          obtain ⟨ o, r, id, c ⟩ := arr[j]
           simp
           intros h_ro_eq
           subst h_ro_eq
@@ -229,14 +229,14 @@ theorem loopInv_YjsLt' {current} offset (arr : Array (YjsItem A)) (newItem : Yjs
             have hlt : YjsLt' (A := A) arr[j] arr[roIdx] := by
               rw [h_ro_in]
               generalize heq : arr[j] = arrj at *
-              obtain ⟨ o, r, id, c, d ⟩ := arrj
+              obtain ⟨ o, r, id, c ⟩ := arrj
               simp at h_ro_eq
               subst h_ro_eq
               exists 1
-              have harrin : ArrSet arr.toList (YjsItem.mk o (YjsPtr.itemPtr ro) id c d) := by
+              have harrin : ArrSet arr.toList (YjsItem.mk o (YjsPtr.itemPtr ro) id c) := by
                 rw [<-heq]
                 simp [ArrSet]
-              apply YjsLt.ltRightOrigin (d := d)
+              apply YjsLt.ltRightOrigin
               apply YjsLeq.leqSame
 
             have hltj : j < arr.size := by
@@ -269,9 +269,9 @@ theorem loopInv_YjsLt' {current} offset (arr : Array (YjsItem A)) (newItem : Yjs
         apply findPtrIdx_getElem; assumption
       apply findPtrIdx_lt_YjsLt' _ _ _ harrinv heq hrightIdx hlt
 
-    obtain ⟨ o, r, id, c, d ⟩ := newItem
+    obtain ⟨ o, r, id, c ⟩ := newItem
     generalize arr[j] = item at *
-    obtain ⟨ oo, or, oid, oc, od ⟩ := item
+    obtain ⟨ oo, or, oid, oc ⟩ := item
     simp at h_origin_eq hlt_ro hlt_ro'
     rw [h_origin_eq]
     rw [h_origin_eq] at hlt_ro'
@@ -316,7 +316,7 @@ theorem loopInv_YjsLt' {current} offset (arr : Array (YjsItem A)) (newItem : Yjs
 
         have hsize : o.size < arr[j].size := by
           revert h_o_eq
-          obtain ⟨ o, r, id, c, d ⟩ := arr[j]
+          obtain ⟨ o, r, id, c ⟩ := arr[j]
           simp
           intros h_o_eq
           subst h_o_eq
@@ -349,14 +349,14 @@ theorem loopInv_YjsLt' {current} offset (arr : Array (YjsItem A)) (newItem : Yjs
             apply getElem_YjsLt'_index_lt arr oIdx j harrinv (by omega) (by omega)
             rw [<-h_o_eq]
             generalize heq : arr[j] = arrj at *
-            obtain ⟨ o, r, id, c, d ⟩ := arrj
+            obtain ⟨ o, r, id, c ⟩ := arrj
             simp
             apply YjsLt'.ltOrigin
             apply YjsLeq'.leqSame
           omega
 
     generalize heq : arr[j] = arrj at *
-    obtain ⟨ o, r, id, c, d ⟩ := arrj
+    obtain ⟨ o, r, id, c ⟩ := arrj
     apply YjsLt'.ltOrigin (A := A)
     simp at hlt_ro
     apply YjsLeq'.leqLt; assumption
@@ -504,7 +504,7 @@ theorem dest_lt_YjsLt'_preserve {A : Type} [inst : DecidableEq A] (newItem : Yjs
       have heq : newItem.origin = other.origin := by
         apply findPtrIdx_eq_ok_inj _ _ heqleft hoLeftIdx
       rw [<-heq]
-      obtain ⟨ o, r, id, c, d ⟩ := newItem
+      obtain ⟨ o, r, id, c ⟩ := newItem
       apply YjsLt'.ltOrigin
       simp
       exists 0; apply YjsLeq.leqSame
@@ -535,11 +535,11 @@ theorem dest_lt_YjsLt'_preserve {A : Type} [inst : DecidableEq A] (newItem : Yjs
           | itemPtr otherOrigin =>
             have ⟨  k, _, h_otherOrigin_arr_k⟩ : ∃(k : ℕ) (h : k < arr.size), arr[k] = otherOrigin := by
               have h_otherOrigin_in_arr : ArrSet arr.toList (YjsPtr.itemPtr otherOrigin) := by
-                obtain ⟨ o, r, id, c, d ⟩ := other
+                obtain ⟨ o, r, id, c ⟩ := other
                 -- rw [heq] at h_other_origin_eq
                 simp at h_other_origin_eq
                 subst o
-                apply harrinv.closed.closedLeft (YjsPtr.itemPtr otherOrigin) r id c d
+                apply harrinv.closed.closedLeft (YjsPtr.itemPtr otherOrigin) r id c
                 rw [<-heq]
                 simp [ArrSet]
               simp [ArrSet] at h_otherOrigin_in_arr
@@ -557,7 +557,7 @@ theorem dest_lt_YjsLt'_preserve {A : Type} [inst : DecidableEq A] (newItem : Yjs
             have otherOrigin_lt : YjsLt' (A := A) otherOrigin arr[(leftIdx + (1 + ↑i)).toNat] := by
               rw [<-h_other_origin_eq]
               generalize h_other_eq : arr[(leftIdx + (1 + ↑i)).toNat] = other at *
-              obtain ⟨ o, r, id, c, d ⟩ := other
+              obtain ⟨ o, r, id, c ⟩ := other
               apply YjsLt'.ltOrigin
               subst other; apply YjsLeq'.leqSame
             have h_lt : k < (leftIdx + (1 + ↑i)).toNat := by
@@ -813,13 +813,13 @@ theorem nDest_geq_i_lt_current_arr_i_origin_eq_newItem_origin_or_arr_nDest_lt_ar
               apply YjsLeq'_findPtrIdx_leq _ _ _ _ _ harrinv _ _ hleq hoLeftIdx; try assumption
               rw [h_arr_nDest_origin_eq_newItem_origin]
               assumption
-              . obtain ⟨ o, r, id, c, d ⟩ := other; simp
-                apply harrinv.closed.closedLeft o r id c d
+              . obtain ⟨ o, r, id, c ⟩ := other; simp
+                apply harrinv.closed.closedLeft o r id c
                 rw [<-heq_other_arr_j]
                 simp [ArrSet]
               . generalize h_eq : arr[nDest.toNat] = arr_nDest at *
-                obtain ⟨ o, r, id, c, d ⟩ := arr_nDest; simp
-                apply harrinv.closed.closedLeft o r id c d
+                obtain ⟨ o, r, id, c ⟩ := arr_nDest; simp
+                apply harrinv.closed.closedLeft o r id c
                 rw [<-h_eq]
                 simp [ArrSet]
 
@@ -1000,9 +1000,9 @@ theorem isDone_true_newItem_lt_item {A : Type} [inst : DecidableEq A] (newItem :
   have harr_other : ArrSet arr.toList (YjsPtr.itemPtr other) := by
     subst other; simp [ArrSet]
   have harr_other_origin : ArrSet arr.toList other.origin := by
-    obtain ⟨ o, r, id, c, d ⟩ := other
+    obtain ⟨ o, r, id, c ⟩ := other
     simp
-    apply harrinv.closed.closedLeft o r id c d
+    apply harrinv.closed.closedLeft o r id c
     rw [<-heq]
     simp [ArrSet]
   -- cases Nat.lt_or_ge (i + 1) ((rightIdx - leftIdx).toNat - 1) with
@@ -1107,8 +1107,8 @@ theorem isDone_true_newItem_lt_item {A : Type} [inst : DecidableEq A] (newItem :
           simp at h_contra
       subst h_oLeftIdx_eq_leftIdx h_oRightIdx_eq_rightIdx
       apply YjsLt'.ltConflict
-      obtain ⟨ o, r, id, c, d ⟩ := newItem
-      obtain ⟨ o', r', id', c', d' ⟩ := other
+      obtain ⟨ o, r, id, c ⟩ := newItem
+      obtain ⟨ o', r', id', c' ⟩ := other
       have h_o_eq_o' : o = o' := by
         simp at *
         apply findPtrIdx_eq_ok_inj _ _ heqleft hoLeftIdx
@@ -1160,9 +1160,9 @@ theorem isDone_true_newItem_lt_item {A : Type} [inst : DecidableEq A] (newItem :
         obtain ⟨ _, horigin_consistent ⟩ := horigin_consistent
         apply not_ptr_lt_first hclosed at horigin_consistent <;> try assumption
         contradiction
-        obtain ⟨ o, r, id, c, d ⟩ := newItem
+        obtain ⟨ o, r, id, c ⟩ := newItem
         simp
-        apply hclosed.closedLeft o r id c d
+        apply hclosed.closedLeft o r id c
         simp [ArrSet]
       | last =>
         simp [findPtrIdx] at heqright
@@ -1172,7 +1172,7 @@ theorem isDone_true_newItem_lt_item {A : Type} [inst : DecidableEq A] (newItem :
         . cases hitem; simp
         . contradiction
     subst hitem
-    obtain ⟨ o, r, id, c, d ⟩ := newItem
+    obtain ⟨ o, r, id, c ⟩ := newItem
     simp
     apply YjsLt'.ltRightOrigin
     apply YjsLeq'.leqSame
@@ -1307,10 +1307,10 @@ theorem loopInv_preserve1
     subst other
     simp [ArrSet]
   have h_in_other_origin : ArrSet (newItem :: arr.toList) other.origin := by
-    obtain ⟨ o, r, id, c, d ⟩ := other
-    apply hclosed.closedLeft _ _ _ _ _ h_in_other
+    obtain ⟨ o, r, id, c ⟩ := other
+    apply hclosed.closedLeft _ _ _ _ h_in_other
   have h_other_origin_lt : YjsLt' (A := A) other.origin other := by
-    obtain ⟨ o, r, id, c, d ⟩ := other
+    obtain ⟨ o, r, id, c ⟩ := other
     simp
     apply YjsLt'.ltOrigin
     apply YjsLeq'.leqSame
@@ -1785,7 +1785,7 @@ theorem YjsArrInvariant_integrate (input : IntegrateInput A) (arr newArr : Array
     constructor
     . simp
       intros i h_i_lt h_i_lt_size
-      obtain ⟨ o, r, id, c, d ⟩ := newItem
+      obtain ⟨ o, r, id, c ⟩ := newItem
       apply YjsLt'.ltOrigin
       simp at *
 
@@ -1829,7 +1829,7 @@ theorem YjsArrInvariant_integrate (input : IntegrateInput A) (arr newArr : Array
             have heq : arr[rightIdx.toNat] = newItem.rightOrigin := by
               apply findPtrIdx_lt_size_getElem heqright' (by omega)
             rw [heq]
-            obtain ⟨ o, r, id, c, d ⟩ := newItem
+            obtain ⟨ o, r, id, c ⟩ := newItem
             apply YjsLt'.ltRightOrigin
             apply YjsLeq'.leqSame
       | some offset0 =>
@@ -1917,3 +1917,16 @@ theorem YjsArrInvariant_integrateSafe (input : IntegrateInput A) (newItem : YjsI
   . rw [<-isClockSafe_maximalId harrinv.unique h_newItem_def] at *
     apply YjsArrInvariant_integrate input arr newArr harrinv h_newItem_def h_valid (by assumption) hintegrate
   . cases hintegrate
+
+theorem YjsStateInvariant_insert (arr newArr : YjsState A) (input : IntegrateInput A) :
+  YjsStateInvariant arr
+  → input.toItem arr.items = Except.ok newItem
+  → newItem.isValid
+  → arr.insert input = Except.ok newArr
+  → YjsStateInvariant newArr := by
+  intros hstateinv h_newItem_def h_valid h_insert
+  simp [YjsStateInvariant, YjsState.insert] at *
+  generalize heq : integrateSafe input arr.items = result at h_insert
+  obtain ⟨ _ ⟩ | ⟨ result ⟩ := result; cases h_insert
+  simp at *
+  grind [YjsArrInvariant_integrateSafe]
